#+OPTIONS: TOC:nil num:nil
#+TITLE: Project 1: Python Truth Tables
#+AUTHOR: Christian Johnson & Aidan Andersen
#+latex_header: \usepackage{amsmath}
#+latex_header: \usepackage{listings}
#+latex_header: \lstset{frame=single, breaklines=true}

#+begin_export latex
\newpage
#+end_export

* Python                                                          :noexport:
#+begin_src python :session DP1

  import pandas as pd
  import io
  from sympy import *

  def ConvertToLatex(df, alignment="c"):
      numcolumns=df.shape[1]
      numRows=df.shape[0]
      output=io.StringIO()
      colFormat=("%s|%s" % (alignment, alignment*numcolumns))
      #Write Header
      output.write("\\begin{tabular}{%s}\n" % colFormat)
      columnLabels=["\\textbf{%s}" % label for label in df.columns]
      output.write(" & %s\\\\\\hline\n" % " & ".join(columnLabels))
      # Date Lines
      for i in range(numRows):
          output.write("\\textbf{%s} & %s\\\\\n"
                       % (df.index[i], " & ".join([str(val) for val in df.iloc[i]])))

      # Write footer
      output.write("\\end{tabular}")
      return output.getvalue()                   

#+end_src

#+RESULTS:
: None

* Proof 1
#+begin_export latex
$p\lor(\lnot q)$\newline
$(t\lor s)\implies(p\lor r)$\newline
$(\lnot r)\lor(t\lor s)$\newline
$\underline{p\implies(t\lor s)}$\newline
$(p\land r)\implies(q\lor r)$\newline\newline
#+end_export
This simplifies to:
#+begin_export latex
\newline
p\lor(\lnot q)\newline
p\implies(p\lor r)\newline
\underline{p\implies(t\lor s)}\newline
(p\land r)\implies (q\lor r)
\newline\newline
\textbf{Given hypotheses:}
\newline
\indent\textbf{1. } $$p\lor (\lnot q)$$ \\
\indent\textbf{2. } $(t\lor s) \implies (p\lor r)$\\
\indent\textbf{3.} $(\lnot r) \lor (t\lor s)$\\
\indent\textbf{4.} $p \implies (q\lor r)$\\
\newline
\textbf{Claim:} $(p \land r) \implies (q\lor r)$\newline
\newline
\textbf{Proof:}
\begin{itemize}
\item Assume $p \land r$. \textit{(Claim)}
\item From 1., we have $p$. \textit{(Conjunction elimination)}
\item Apply hypothesis 4 to $p$, which implies $q\lor r$. \textit{(Modus Ponens)}
\item Since $r$ is also true, $q\lor r$ holds. \textit{(Disjunctive Syllogism)}
\item Therefore, $(p\land r)\implies (q\lor r)$ is established
\end{itemize}
\newline\newline
This conclusion can be shown in the truth table on the next 2 pages.
\newpage
\begin{lstlisting}[language=Python]
  variables=['p', 'q', 'r', 's', 't']
  expression1=lambda p,r: p and r
  expression2=lambda q,r: q or r
  expression3=lambda p,q,r: Implies(p&r,q|r)
  data=[]

  for p in (True, False):
      for q in (True, False):
          for r in (True, False):
              for t in (True, False):
                  for s in (True, False):
                      result1=expression1(p,r)
                      result2=expression2(q,r)
                      result3=expression3(p,q,r)
                      data.append([p,q,r,t,s,result1,result2,result3])
  df=pd.DataFrame(data, columns=['p','q','r','s','t','p and r','q or r','(p and r) implies (q or r)'])
  ConvertToLatex(df)
\end{lstlisting}
#+end_export


#+begin_src python :results file :file Project1Export1.tex :exports none :session DP1

    variables=['p', 'q', 'r', 's', 't']
    expression1=lambda p,r: p and r
    expression2=lambda q,r: q or r
    expression3=lambda p,q,r: Implies(p&r,q|r)
    data=[]

    for p in (True, False):
        for q in (True, False):
            for r in (True, False):
                for t in (True, False):
                    for s in (True, False):
                        result1=expression1(p,r)
                        result2=expression2(q,r)
                        result3=expression3(p,q,r)
                        data.append([p,q,r,t,s,result1,result2,result3])
    df=pd.DataFrame(data, columns=['p','q','r','s','t','p and r','q or r','(p and r) implies (q or r)'])
    ConvertToLatex(df)


#+end_src

#+RESULTS:
[[file:Project1Export1.tex]]

#+begin_export latex
\newpage
\hspace{-2cm}\input{Project1Export1.tex}
\newpage
#+end_export

* Proof 2

#+begin_export latex
$p\lor(\lnot q)$\\
$(t\lor s)\implies(p\lor r)$ \\
$(\lnot r)\lor(t\lor s)$ \\
$\underline{p\iff(t\lor s)}$\\
$(q\lor r)\implies(p\lor r)$\\
\newline\newline
#+end_export
This can be simplified to:
#+begin_export latex
\newline
$p\lor(\lnot q)$ \\
$p\implies (p\lor r)$ \\
$\underline{(\lnot r)\lor(t\lor s)}$ \\
$(q\lor r)\implies(p\lor r)$\\
\newline\newline
\textbf{Given hypotheses:}\newline
\indent\textbf{1.} $p\lor(\lnot q)$\\
\indent\textbf{2.} $p\implies(p\lor r)$\\
\indent\textbf{3.} $(\lnot r)\lor(t\lor s)$\\
\textbf{Claim:} $(q\lor r)\implies(p\lor r)$
\textbf{Proof:}\newline
\begin{itemize}
\item Assume $q\lor r$.  \textit{(Claim)}
\item From 1, we know p, since 
#+end_export

